% !TeX root = ./TMA02.tex

\begin{table}[!htp]\centering
\begin{tabular}{lrr|cr}\toprule
$v_1$ &$v_2$ &$v_3$ &$f(v_1, v_2, v_3)$ \\\midrule
0 &0 &0 &0 \\
1 &0 &0 &1 \\
0 &1 &0 &1 \\
1 &1 &0 &0 \\
0 &0 &1 &1 \\
1 &0 &1 &0 \\
0 &1 &1 &1 \\
1 &1 &1 &1 \\
\bottomrule
\end{tabular}
\caption{Truth table for function $f:V(3,2) \rightarrow V(1,2)$.}\label{tab:4}
\end{table}
We obtain an expression for $f(v_1, v_2, v_3)$ as a Boolean multinomial in three Boolean variables as follows.

Making use of: $x\lor y = x + y +xy$; $x + x = 0$; $xx=x$; and $x + x=0$ in $GF(2)$, gives
\begin{align}
f(v_1, v_2, v_3) &=      v_1  \bar{v_2} \bar{v_3}\; \lor
                    \bar{v_1}      v_2  \bar{v_3}\; \lor
                    \bar{v_1} \bar{v_2}      v_3 \; \lor
                    \bar{v_1}      v_2       v_3 \; \lor
                         v_1       v_2       v_3\nonumber\\
              &= \bar{v_1}v_3(v_2 + \bar{v_2}) + 
                 \bar{v_1}v_2(v_3 + \bar{v_3}) +
                      v_2 v_3(v_1 + \bar{v_1}) + 
                      v_1\bar{v_2}\bar{v_3}\nonumber \\
              &= \bar{v_1}v_3 + 
                 \bar{v_1}v_2 +
                      v_2 v_3 + 
                      v_1\bar{v_2}\bar{v_3}\nonumber \\
              &= (1 + v_1)v_3 + 
                 (1 + v_1)v_2 +
                      v_2 v_3 + 
                      v_1(1 + v_2)(1 + v_3)\nonumber \\
              &= v_3 + v_1v_3 + 
                 v_2 + v_1v_2 +
                      v_2 v_3 + 
                      v_1 + v_1v_3 + v_1v_2 + v_1v_2v_3\nonumber\\
\label{bool:1}             &= v_1 +v_2 + v_3 + v_2v_3 +v_1v_2v_3
\end{align}
Check:

\begin{table}[!htp]\centering
\begin{tabular}{lcc|c|c|cc}\toprule
$v_1$ &$v_2$ &$v_3$ &$v_2v_3$ &$v_1v_2v_3$ &$v_1+v_2+v_3+v_2v_3+v_1v_2v_3$ \\\midrule
0 &0 &0 &0 &0 &0 \\
1 &0 &0 &0 &0 &1 \\
0 &1 &0 &0 &0 &1 \\
1 &1 &0 &0 &0 &0 \\
0 &0 &1 &0 &0 &1 \\
1 &0 &1 &0 &0 &0 \\
0 &1 &1 &1 &0 &1 \\
1 &1 &1 &1 &1 &1 \\
\bottomrule
\end{tabular}
\caption{Truth Table for \eqref{bool:1}}\label{tab:5}
\end{table}
The last columns of Table~\ref{tab:5} and Table~\ref{tab:4} are in agreement. Thus, $f(v_1, v_2, v_3) = v_1+v_2+v_3+v_2v_3+v_1v_2v_3$.

